in Prop gespielt

Code/DFA_Prop.v
@@ -1,3 +1,5 @@
+Require Import Bool.
+Load DFA_Def.
 
 (* Erweiterte Überführungsfunktion über *)
 Theorem delta_hat_append : forall (xs : list Sigma) (ys : list Sigma) (q : Q),
@@ -11,3 +13,40 @@ Proof.
     intros.
     apply IHxs.
 Qed.
+
+(*i*)
+(*
+Inductive Konf_DFA_step : Konf_DFA -> Konf_DFA -> Type :=
+ | one_step : forall (q : Q) (p : Q) (a : Sigma) (w : list Sigma) (eq : (delta q a) = p), 
+                                    Konf_DFA_step (q, (cons a w)) (p, w).
+Inductive Konf_rel_DFA : Konf_DFA -> Konf_DFA -> Type :=
+  | refl    : forall (K : Konf_DFA), Konf_rel_DFA K K
+  | step  : forall (K L M : Konf_DFA),
+                                    Konf_rel_DFA K L ->
+                                    Konf_DFA_step L M ->
+                                    Konf_rel_DFA K M.
+*)
+
+(*ii*)
+(*(|--) Konf_DFA -> (Konf_DFA -> Prop)*)
+Inductive Konf_DFA_step_bool : Konf_DFA -> (Konf_DFA -> Prop) :=
+ | one_step_bool : forall (q : Q) (p : Q) (a : Sigma) (w : list Sigma) (eq : (delta q a) = p),
+                                    Konf_DFA_step_bool (q, (cons a w)) (p, w).
+(*(|--* ) Konf_DFA -> (Konf_DFA -> Prop)*)
+Inductive Konf_rel_DFA_bool : Konf_DFA -> (Konf_DFA -> Prop) :=
+  | refl_bool    : forall (K : Konf_DFA), Konf_rel_DFA_bool K K
+  | step_bool  : forall (K L M : Konf_DFA),
+                                    Konf_rel_DFA_bool K L ->
+                                    Konf_DFA_step_bool L M ->
+                                    Konf_rel_DFA_bool K M.
+
+(*iii*)
+(*dec_Konf_DFA_step : (K1 : Konf_DFA) -> (K2 : Konf_DFA) -> Dec (K1 |-- K2)*)
+(*dec_Konf_DFA : (K1 : Konf_DFA) -> (K2 : Konf_DFA) -> Dec (K1 |--* K2)*)
+
+(*(ii) <=> (i) /\ (iii)*)
+(*Über die Entscheidbarkeit zeigen, dass Konf_DFA -> Type = Konf_DFA -> Prop*)
+Theorem Konf_eq : forall (conf: Konf_DFA), Konf_DFA_step_bool -> Konf_DFA_step.
+Proof.
+intros.
+destruct Konf_DFA_step.
